More lemmas about the LR

theories/L6_PCPS/Heap/log_rel_post_cc.v
@@ -24,7 +24,7 @@ Module LogRelPostCC (H : Heap).
              (fR : fun_body_rel) : Prop :=
     match v1, v2 with
     | FunPtr B1 f1, FunPtr B2 f2 =>
-      forall rho1 ft1 xs1 e1 vs1 vs2 b,        
+      forall H1 H2 rho1 ft1 xs1 e1 vs1 vs2 b,        
         find_def f1 B1 = Some (ft1, xs1, e1) ->
         setlist xs1 vs1 (def_funs B1 B1 (M.empty _)) = Some rho1 ->
 
@@ -66,13 +66,29 @@ Module LogRelPostCC (H : Heap).
       edestruct Hfun as [ft2 [xs2 [e2 [rho2 [Hdef2 [Hset2 Hrel]]]]]]; try eassumption.
       repeat eexists; eauto. eapply Hyp. eassumption.
   Qed. 
-      
-  Definition val_rel := val_log_rel big_step_GC_cc big_step_GC_cc no_clos_rel fun_ptr_rel. 
+
+  Instance Proper_clos_rel_impl : forall P Q b b1 H1 b2 H2,
+      Proper ((pointwise_lifting impl fun_body_args) ==> (pointwise_lifting impl val_rel_args) ==> impl)
+             (no_clos_rel P Q b b1 H1 b2 H2).
+  Proof. clear; now firstorder. Qed. 
+
+  Instance Proper_fun_rel_impl : forall  P Q b v1 H1 v2 H2,
+      Proper ((pointwise_lifting impl fun_body_args) ==> impl) (fun_ptr_rel P Q b v1 H1 v2 H2).
+  Proof.
+    intros. intros P1 P2 Hyp.
+    unfold fun_ptr_rel. destruct v1; destruct v2; unfold impl; eauto.
+    intros Hfun. intros.
+    edestruct Hfun as [ft2 [xs2 [e2 [rho2 [Hdef2 [Hset2 Hrel]]]]]]; try eassumption.
+    repeat eexists; eauto. eapply Hyp. eassumption.
+  Qed. 
+
+  Definition val_rel := val_log_rel' big_step_GC_cc big_step_GC_cc no_clos_rel fun_ptr_rel. 
   Definition exp_rel := exp_log_rel val_rel big_step_GC_cc big_step_GC_cc.
   Definition var_rel := var_log_rel' big_step_GC_cc big_step_GC_cc no_clos_rel fun_ptr_rel.
   Definition env_rel := env_log_rel_P' big_step_GC_cc big_step_GC_cc no_clos_rel fun_ptr_rel.
   Definition heap_rel := heap_log_rel val_rel.
 
+  
   Definition val_rel' (k : nat)  (j : nat) (IP : GIInv) (P : GInv) (b : Inj) (r1 r2 : ans) : Prop :=
     match r1, r2 with
     | OOT, OOT => True (* Both programs timeout *)
@@ -87,7 +103,7 @@ Module LogRelPostCC (H : Heap).
         | _, _ => False
         end
       | FunPtr B1 f1, FunPtr B2 f2 =>
-        forall rho1 ft1 xs1 e1 vs1 vs2 b,        
+        forall H1 H2 rho1 ft1 xs1 e1 vs1 vs2 b,        
           find_def f1 B1 = Some (ft1, xs1, e1) ->
           setlist xs1 vs1 (def_funs B1 B1 (M.empty _)) = Some rho1 ->
 
@@ -110,12 +126,25 @@ Module LogRelPostCC (H : Heap).
       end
     | _, _ => False
     end.
+  
+  
+  Notation "p1 ⪯ ^ ( k ; j ; P1 ; P2 ; P3 ; P4 ) p2" :=
+    (exp_rel k j P1 P2 P3 P4 p1 p2) (at level 70, no associativity).
 
-  Opaque val_log_rel val_log_rel'. 
+  Notation "p1 ≺ ^ ( k ; j ; IP ; P ; b ) p2" :=
+    (val_rel k j IP P b p1 p2) (at level 70, no associativity).
+  
+  Notation "p1 ⋞ ^ ( R ; k ; j ; IP ; P ; b ) p2" :=
+    (env_rel R k j IP P b p1 p2) (at level 70, no associativity).
+
+  Notation "S |- H1 ≼ ^ ( k ; j ; IP ; P ; b ) H2" :=
+    (heap_rel S k j IP P b H1 H2) (at level 70, no associativity).
+
   
   Lemma val_rel_eq k j IP P b r1 r2 :
     val_rel k j IP P b r1 r2 <-> val_rel' k j IP P b r1 r2.
   Proof.
+    unfold val_rel. 
     destruct k; destruct j; 
       destruct r1 as [[[l1 | lf1 f1] H1] |]; destruct r2 as [[[l2 | lf2 f2] H2] |];
         try (now split; intros; contradiction);
@@ -141,37 +170,37 @@ Module LogRelPostCC (H : Heap).
       exfalso; omega.
       
       intros Hyp. intros.
-      edestruct Hyp as [ft2 [xs2 [e2 [Hdef2 [Hset2 Hrel]]]]]; try eassumption.
-      do 4 eexists; repeat split; eauto.
-
+      edestruct Hyp as [ft2 [xs2 [e2 [rho2 [Hdef2 [Hset2 Hrel]]]]]]; try eassumption.
+      do 4 eexists; repeat split; eauto. exfalso; omega. exfalso; omega. 
     - split.
-      + simpl. intros [Hyp1 Hyp2]. split; eauto. 
+      + intros [Hyp1 Hyp2]. split; eauto. 
         destruct (get l1 H1) as [b1|]; destruct (get l2 H2) as [b2|]; try now eauto. 
         destruct b1 as [c1 vs1 | v1 v2 | ]; try now eauto.
         destruct b2 as [c2 vs2 | v1' v2' | ]; try contradiction.
         destruct Hyp2 as [Hyp2 Hyp3]. split; eauto.
         eapply Forall2_monotonic; [| eassumption ].
         intros v1 v2 Hyp i Hlt. 
-        replace i with (j - (j - i)) by omega. eapply Hyp. omega.
-      + simpl. intros [Hyp1 Hyp2]. split; eauto. 
+        replace i with (j - (j - i)) by omega. unfold val_rel. rewrite <- val_log_rel_eq; tci.
+        eapply Hyp. omega.
+      + intros [Hyp1 Hyp2]. split; eauto. 
         destruct (get l1 H1) as [b1|]; destruct (get l2 H2) as [b2|]; try now eauto. 
         destruct b1 as [c1 vs1 | v1 v2 | ]; try now eauto.
         destruct b2 as [c2 vs2 | v1' v2' | ]; try contradiction.
         destruct Hyp2 as [Hyp2 Hyp3]. split; eauto.
         eapply Forall2_monotonic; [| eassumption ].
         intros v1 v2 Hyp i Hlt.
-        replace (j - (j - i)) with i by omega. eapply Hyp. omega.
-    - simpl. split. 
-      intros Hyp. intros.
-      edestruct Hyp as [ft2 [xs2 [e2 [Hdef2 [Hset2 Hrel]]]]]; try eassumption.
+        rewrite val_log_rel_eq; tci.
+        eapply Hyp. omega.
+    - split. intros Hyp. simpl. intros.
+      edestruct Hyp as [ft2 [xs2 [e2 [rho2 [Hdef2 [Hset2 Hrel]]]]]]; try eassumption.
       do 4 eexists; repeat split; eauto. exfalso. omega. 
       exfalso; omega.
       
-      intros Hyp. intros.
+      intros Hyp. simpl. intros.
       edestruct Hyp as [ft2 [xs2 [e2 [Hdef2 [Hset2 Hrel]]]]]; try eassumption.
-      do 4 eexists; repeat split; eauto.
+      do 4 eexists; repeat split; eauto; exfalso; omega.
     - split.
-      + simpl. intros [Hyp1 Hyp2]. split; eauto. 
+      + intros [Hyp1 Hyp2]. split; eauto. 
         destruct (get l1 H1) as [b1|]; destruct (get l2 H2) as [b2|]; try now eauto. 
         destruct b1 as [c1 vs1 | v1 v2 | ]; try now eauto.
         destruct b2 as [c2 vs2 | v1' v2' | ]; try contradiction.
@@ -183,92 +212,103 @@ Module LogRelPostCC (H : Heap).
         destruct b2 as [c2 vs2 | v1' v2' | ]; try contradiction.
         destruct Hyp2 as [Hyp2 Hyp3]. split; eauto.
         eapply Forall2_monotonic; [| eassumption ]. intros. omega.
-    - simpl. split. 
-      + intros Hyp. intros.  
+    - split. 
+      + intros Hyp. simpl; intros.  
         edestruct Hyp as [ft2 [xs2 [rho2 [e2 [Hdef2 [Hset2 Hrel]]]]]]; try eassumption.
         do 4 eexists; split; [| split ]; eauto. intros i Hlt Hall.
         assert (Hieq : k - (k - i) = i) by omega. 
         split.  
         eapply Hrel; eauto. intros j.   
         eapply Forall2_monotonic; [| now eapply (Hall j)  ].
-        intros v1 v2 Hyp'. rewrite Hieq. now eapply Hyp'.
+        intros v1 v2 Hyp'. rewrite val_log_rel_eq; tci. now eapply Hyp'.
         
-        setoid_rewrite <- Hieq. eapply Hrel; eauto. intros j. 
-        eapply Forall2_monotonic; [| now eapply (Hall j)  ].
-        intros v1 v2 Hyp'. rewrite Hieq. eassumption.
-      + intros Hyp. intros. 
+        setoid_rewrite <- Hieq.
+        unfold val_rel. setoid_rewrite <- val_log_rel_eq; tci. eapply Hrel; eauto. omega.
+        intros j. eapply Forall2_monotonic; [| now eapply (Hall j) ].
+        intros v1 v2 Hyp'. rewrite Hieq. rewrite val_log_rel_eq; tci.
+      + intros Hyp. simpl. intros. 
         edestruct Hyp as [ft2 [xs2 [rho2 [e2 [Hdef2 [Hset2 Hrel]]]]]]; try eassumption.
         do 4 eexists; split; [| split ]; eauto. intros i Hlt Hall.
         assert (Hieq : k - (k - i) = i) by omega. 
         split. 
         eapply Hrel; eauto. intros j.  
         eapply Forall2_monotonic; [| now eapply (Hall j)  ].
-        intros v1 v2 Hyp'. rewrite <- Hieq. now eapply Hyp'.
-        
-        setoid_rewrite  Hieq. eapply Hrel; eauto. intros j. 
+        intros v1 v2 Hyp'. unfold val_rel.
+        rewrite <- val_log_rel_eq; tci. now eapply Hyp'.
+
+        setoid_rewrite val_log_rel_eq; tci. 
+        eapply Hrel; eauto. intros j. 
         eapply Forall2_monotonic; [| now eapply (Hall j)  ].
-        intros v1 v2 Hyp'. rewrite <- Hieq. eassumption.
+        intros v1 v2 Hyp'. unfold val_rel.
+        rewrite <- val_log_rel_eq; tci.
     - split.
-      + simpl. intros [Hyp1 Hyp2]. split; eauto. 
+      + intros [Hyp1 Hyp2]. split; eauto. 
         destruct (get l1 H1) as [b1|]; destruct (get l2 H2) as [b2|]; try now eauto. 
         destruct b1 as [c1 vs1 | v1 v2 | ]; try now eauto.
         destruct b2 as [c2 vs2 | v1' v2' | ]; try contradiction.
         destruct Hyp2 as [Hyp2 Hyp3]. split; eauto.
         eapply Forall2_monotonic; [| eassumption ].
         intros v1 v2 Hyp i Hlt. 
-        replace i with (j - (j - i)) by omega. eapply Hyp. omega.
-      + simpl. intros [Hyp1 Hyp2]. split; eauto. 
+        replace i with (j - (j - i)) by omega. unfold val_rel.
+        rewrite <- val_log_rel_eq; tci. eapply Hyp. omega. 
+      + intros [Hyp1 Hyp2]. split; eauto. 
         destruct (get l1 H1) as [b1|]; destruct (get l2 H2) as [b2|]; try now eauto. 
         destruct b1 as [c1 vs1 | v1 v2 | ]; try now eauto.
         destruct b2 as [c2 vs2 | v1' v2' | ]; try contradiction.
         destruct Hyp2 as [Hyp2 Hyp3]. split; eauto.
         eapply Forall2_monotonic; [| eassumption ].
-        intros v1 v2 Hyp i Hlt.
-        replace (j - (j - i)) with i by omega. eapply Hyp. omega.
-    - simpl. split. 
-      + intros Hyp. intros. 
+        intros v1 v2 Hyp i Hlt. rewrite val_log_rel_eq; tci.
+        eapply Hyp; eauto.        
+    - split. 
+      + intros Hyp. simpl. intros. 
         edestruct Hyp as [ft2 [xs2 [rho2 [e2 [Hdef2 [Hset2 Hrel]]]]]]; try eassumption.
         do 4 eexists; split; [| split ]; eauto. intros i Hlt Hall.
-        assert (Hieq : k - (k - i) = i) by omega. 
         split. 
         eapply Hrel; eauto. intros j'.  
         eapply Forall2_monotonic; [| now eapply (Hall j')  ].
-        intros v1 v2 Hyp'. rewrite Hieq. now eapply Hyp'. 
-        
-        setoid_rewrite <- Hieq. eapply Hrel; eauto. intros j'. 
-        eapply Forall2_monotonic; [| now eapply (Hall j')  ].
-        intros v1 v2 Hyp'. rewrite Hieq. eassumption.
-      + intros Hyp. intros. 
-        edestruct Hyp as [ft2 [xs2 [rho2 [e2 [Hdef2 [Hset2 Hrel]]]]]]; try eassumption.
-        do 4 eexists; split; [| split ]; eauto. intros i Hlt Hall.
-        assert (Hieq : k - (k - i) = i) by omega. 
-        split. 
-        eapply Hrel; eauto. intros j'.  
-        eapply Forall2_monotonic; [| now eapply (Hall j')  ].
-        intros v1 v2 Hyp'. rewrite <- Hieq. now eapply Hyp'. 
-        
-        setoid_rewrite  Hieq. eapply Hrel; eauto. intros j'. 
-        eapply Forall2_monotonic; [| now eapply (Hall j')  ].
-        intros v1 v2 Hyp'. rewrite <- Hieq. eassumption.
+        intros v1 v2 Hyp'. rewrite val_log_rel_eq; tci.
 
-        Grab Existential Variables. exact id. exact id.
+        apply Hyp'; eauto. unfold val_rel. setoid_rewrite <- val_log_rel_eq; tci.          
+        apply Hrel; eauto.
+
+        intros j'. eapply Forall2_monotonic; [| now eapply (Hall j')  ].
+        intros v1 v2 Hyp'. rewrite val_log_rel_eq; tci.
+      + intros Hyp. simpl. intros. 
+        edestruct Hyp as [ft2 [xs2 [rho2 [e2 [Hdef2 [Hset2 Hrel]]]]]]; try eassumption.
+        do 4 eexists; split; [| split ]; eauto. intros i Hlt Hall.
+        assert (Hieq : k - (k - i) = i) by omega. 
+        split. 
+        eapply Hrel; eauto. intros j'.  
+        eapply Forall2_monotonic; [| now eapply (Hall j')  ].
+        intros v1 v2 Hyp'. unfold val_rel. rewrite <- val_log_rel_eq; tci.
+        now eapply Hyp'. setoid_rewrite val_log_rel_eq; tci.          
+        apply Hrel; eauto.
+        
+        intros j'. eapply Forall2_monotonic; [| now eapply (Hall j')  ].
+        intros v1 v2 Hyp'. unfold val_rel. rewrite <- val_log_rel_eq; tci.
+        
+        Grab Existential Variables.
+        eassumption. eassumption. eassumption. eassumption.
+        eassumption. eassumption. eassumption. eassumption.
+        eassumption. eassumption. eassumption. eassumption.        
+
   Qed.
 
   (** * Respects f_eq_subdomain *)
 
-  
-  Lemma val_rel_rename_ext IP P b b' k j r1 r2:
-    val_rel k j IP P b r1 r2 ->
+  Lemma val_rel_rename_ext GIP GP b b' k j r1 r2:
+    r1 ≺ ^ (k ; j ; GIP ; GP ; b) r2 ->
     f_eq_subdomain (reach_ans r1) b b' ->
-    val_rel k j IP P b' r1 r2.
+    r1 ≺ ^ (k ; j ; GIP ; GP ; b') r2.
   Proof with (now eauto with Ensembles_DB).
-    rewrite !val_rel_eq in *. revert k j b b' r1 r2.
+    revert k j b b' r1 r2.
     induction k as [k IHk] using lt_wf_rec1.
     induction j as [j IHj] using lt_wf_rec1.
+    setoid_rewrite val_rel_eq.
     intros b b' [[v1 H1] | ] [[v2 H2] | ] Hres Hfeq; try contradiction; [| now eauto ].
-    destruct v1 as [l1 | lf1 f1]; destruct v2 as [l2 | lf2 f2]; simpl;
-    try contradiction; try (now simpl; eauto).
-    - simpl in Hres. destruct Hres as [Heq Hres]. 
+    destruct v1 as [l1 | lf1 f1]; destruct v2 as [l2 | lf2 f2];
+    try contradiction; try (now simpl; eauto). 
+    - unfold val_rel' in *. destruct Hres as [Heq Hres]. 
       destruct (get l1 H1) as [b1'|] eqn:Hget1; destruct (get l2 H2) as [b2'|] eqn:Hget2;
         (try now eauto);
         try (destruct b1' as [ | | ]; contradiction). 
@@ -278,37 +318,15 @@ Module LogRelPostCC (H : Heap).
       + destruct b1' as [c1 vs1 | [? | B1 f1] [ env_loc1 |] | ]; try contradiction;
           destruct b2' as [c2 vs2 | | ]; try contradiction. 
         destruct Hres as [Hceq Hall]. split; eauto. 
-        eapply Forall2_monotonic_strong; [| eassumption ]. intros x1 x2 Hin1 Hin2 HR i Hlt.
-        rewrite val_rel_eq. eapply IHj. eassumption.
-        rewrite <- val_rel_eq. eapply HR; eauto.
+        eapply Forall2_monotonic_strong; [| eassumption ].
+        intros x1 x2 Hin1 Hin2 HR i Hlt.
+        eapply IHj; eauto. 
         
         eapply f_eq_subdomain_antimon; [| eassumption ].
         rewrite (reach_unfold H1 (val_loc (Loc l1))).
         eapply Included_Union_preserv_r. eapply reach'_set_monotonic.
         simpl. rewrite post_Singleton; [| eassumption ].
         eapply In_Union_list. eapply in_map. eassumption.
-    (* - intros rho1 ft1 xs1 e1 vs1 vs2 Hdef1 Hset1 Hlen. *)
-    (*   edestruct Hres as [ft2 [xs2 [e2 [rho2 [Hdef2 [Hset2 Hrel]]]]]]; try eassumption. *)
-    (*   do 4 eexists. split. eassumption. split. eassumption. intros i Hlt Hall. *)
-    (*   eapply Hrel. eassumption. *)
-    (*   intros j'. *)
-      
-    (*   eapply Forall2_monotonic_strong; [| exact (Hall j') ]. intros x1 x2 Hin1 Hin2 HR. *)
-    (*   rewrite val_rel_eq. eapply IHk. eassumption. *)
-    (*   rewrite <- val_rel_eq. eapply HR; eauto. *)
-    (*   symmetry.  *)
-    (*   eapply f_eq_subdomain_antimon; [| eassumption ]. *)
-    (*   rewrite (reach_unfold H1 (val_loc (Loc l1))). *)
-    (*   eapply Included_Union_preserv_r. eapply reach'_set_monotonic. *)
-    (*   simpl. rewrite post_Singleton; [| eassumption ]. *)
-    (*   eapply In_Union_list. eapply in_map. eassumption. *)
-      
-    (*   ; eauto. exfalso. omega.  *)
-    (*   exfalso; omega. *)
-      
-    (*   intros Hyp. intros. *)
-    (*   edestruct Hyp as [ft2 [xs2 [e2 [Hdef2 [Hset2 Hrel]]]]]; try eassumption. *)
-    (*   do 4 eexists; repeat split; eauto. *)
   Qed.
 
   Lemma var_rel_rename_ext k j IP P b b' H1 H2 rho1 rho2 x y: 
@@ -318,16 +336,15 @@ Module LogRelPostCC (H : Heap).
   Proof with (now eauto with Ensembles_DB).
     intros Hcc Heq v Hget. edestruct Hcc as [l2 [Hget2 Hres]].
     eassumption. eexists; split; eauto.
-    rewrite <- val_log_rel_eq in *; tci.
     eapply val_rel_rename_ext. eassumption.
     eapply f_eq_subdomain_antimon; [| eassumption ].
     eapply reach'_set_monotonic. eapply env_locs_Singleton; try eassumption.
   Qed. 
   
-  Lemma env_rel_rename_ext S k j IP P b b' H1 H2 rho1 rho2 : 
-    env_rel S k j IP P b (H1, rho1) (H2, rho2) ->
+  Lemma env_rel_rename_ext GIP GP S k j b b' H1 H2 rho1 rho2 : 
+    (H1, rho1) ⋞ ^ (S; k; j; GIP; GP; b) (H2, rho2) ->
     f_eq_subdomain (reach' H1 (env_locs rho1 S)) b b' ->
-    env_rel S k j IP P b' (H1, rho1) (H2, rho2).
+    (H1, rho1) ⋞ ^ (S; k; j; GIP; GP; b') (H2, rho2).
   Proof with (now eauto with Ensembles_DB).
     intros Henv Heq x Hin v Hget. 
     eapply var_rel_rename_ext. eapply Henv. 
@@ -339,9 +356,9 @@ Module LogRelPostCC (H : Heap).
 
 
   Lemma heap_rel_rename_ext S k j IP P b b' H1 H2 : 
-    heap_rel S k j IP P b H1 H2 ->
+    S |- H1 ≼ ^ ( k ; j ; IP ; P ; b ) H2 ->
     f_eq_subdomain (reach' H1 S) b b' ->
-    heap_rel S k j IP P b' H1 H2.
+    S |- H1 ≼ ^ ( k ; j ; IP ; P ; b' ) H2.
   Proof with (now eauto with Ensembles_DB).
     intros Hheap Hfeq x Hin.
     eapply val_rel_rename_ext. 
@@ -352,14 +369,353 @@ Module LogRelPostCC (H : Heap).
     eapply Singleton_Included. eassumption.
   Qed.
 
+  Global Instance Proper_val_rel_f_eq k j IP P :
+    Proper (f_eq ==> eq ==> eq ==> iff) (val_rel' k j IP P).
+  Proof.
+    intros ? ? H ? ? ? ? ? ?. subst.
+    split; intros H1.
+    rewrite <- val_rel_eq. eapply val_rel_rename_ext.
+    rewrite val_rel_eq. eassumption.
+    rewrite H. reflexivity.
+    rewrite <- val_rel_eq. eapply val_rel_rename_ext.
+    rewrite val_rel_eq. eassumption.
+    rewrite H. reflexivity.
+  Qed. 
 
-  
+  Global Instance Proper_env_rel_f_eq S k j IP P :
+    Proper (f_eq ==> eq ==> eq ==> iff) (env_rel S k j IP P).
+  Proof.
+    intros ? ? H [? ?] [? ?] Heq [? ?] [? ?] Heq'. inv Heq; inv Heq'.
+    split; intros H1; eapply env_rel_rename_ext.
+    eassumption.
+    rewrite H. reflexivity.
+    eassumption.
+    rewrite H. reflexivity.
+  Qed. 
 
+  Global Instance Proper_heap_rel_f_eq S k j IP P :
+    Proper (f_eq ==> eq ==> eq ==> iff) (heap_rel S k j IP P).
+  Proof.
+    intros ? ? H ? ? Heq ? ? Heq'. subst.
+    split; intros H1; eapply heap_rel_rename_ext.
+    eassumption.
+    rewrite H. reflexivity.
+    eassumption.
+    rewrite H. reflexivity.
+  Qed. 
     
   (** * Logical relation respects heap_equivalence *)  
+
+    Lemma val_rel_res_eq GIP GP (k j : nat) (b' b1 b2 : Inj) (H1 H2 H1' H2' : heap block)
+        (v1 v2 v1' v2' : value) :
+    (Res (v1, H1)) ≺ ^ (k ; j ; GIP ; GP ; b') (Res (v2, H2)) ->
+
+    (v1, H1) ≈_(id, b1) (v1', H1') ->
+    injective_subdomain (reach' H1' (val_loc v1')) b1 ->
+
+    (v2, H2) ≈_(b2, id) (v2', H2') ->
+    injective_subdomain (reach' H2 (val_loc v2)) b2 ->
+    
+    (Res (v1', H1')) ≺ ^ (k ; j ; GIP ; GP ; b2 ∘ b' ∘ b1) (Res (v2', H2')).
+  Proof with now eauto with Ensembles_DB.
+    revert j b' b1 b2 v1 v2 v1' v2' H1 H2 H1' H2'.
+    induction k as [k IHk] using lt_wf_rec1. intros j.
+    induction j as [j IHj] using lt_wf_rec1.
+    intros b' b1 b2 v1 v2 v1' v2' H1 H2 H1' H2'. 
+    destruct v1 as [l1 | lf1 f1]; destruct v2 as [l2 | lf2 f2];
+      try (now intros; contradiction); try (now simpl; eauto).
+    - simpl. 
+      intros [Heq Hcc] (* Hwf1 Hwf2 Hl1 Hl2 *) Hres1 Hr1 Hres2 Hr2. 
+      destruct (get l1 H1) as
+          [[c1 vs1 | | ] | ] eqn:Hget1;
+        destruct (get l2 H2) as
+          [[c2 vs2 | | ] | ] eqn:Hget2; try contradiction.
+      rewrite res_equiv_eq in Hres1, Hres2.
+      destruct v1' as [l1' | lf1' f1']; destruct v2' as [l2' | lf2' f2'];
+      try contradiction.
+      simpl in Hres1, Hres2. 
+      rewrite Hget1 in Hres1. rewrite Hget2 in Hres2.
+      destruct Hres1 as [Heqi1 Hres1].
+      destruct Hres2 as [Heqi2 Hres2]. subst.       
+      destruct (get l1' H1') as [b1'|] eqn:Hget1'; [| contradiction ].
+      destruct (get l2' H2') as [b2'|] eqn:Hget2'; [| contradiction ].
+      destruct b1' as [c1' vs1' | | ]; [| contradiction | contradiction ].
+      destruct b2' as [c2' vs2' | | ]; [| contradiction | contradiction ].
+      
+      destruct Hres1 as [Heqc1 Heqb1].
+      destruct Hres2 as [Heqc2 Heqb2]. subst. 
+      destruct Hcc as [Heqc Hall]; subst. 
+      split. unfold compose. rewrite <- Heqi1. unfold id. rewrite Heqi2.
+      reflexivity.
+      split; eauto.
+      
+      eapply Forall2_vertical_l_strong
+        with (R1 := fun x y => forall i : nat, i < j ->
+                             Res (x, H1) ≺ ^ (k; i; GIP; GP; b2 ∘ b') Res (y, H2')); 
+        [| | now eapply Heqb1 ].
+      
+      * intros.
+        setoid_rewrite val_log_rel_eq; tci. 
+        eapply val_rel_rename_ext;
+          [| rewrite <- (compose_id_neut_l (b2 ∘ b' ∘ b1)); reflexivity ]. 
+        rewrite <- Combinators.compose_assoc.
+        eapply IHj; try eassumption; try reflexivity.
+        eapply H4. eassumption. eassumption. 
+        
+        eapply injective_subdomain_antimon. eassumption.
+        rewrite (reach_unfold _ (val_loc (Loc l1'))).
+        eapply Included_Union_preserv_r.
+        eapply reach'_set_monotonic. simpl. rewrite post_Singleton; [| eassumption ].
+        eapply In_Union_list. eapply in_map. eassumption.
+
+        clear. now firstorder.
+      * eapply Forall2_vertical_r_strong; [| eapply Hall | eassumption ].
+        intros x y z Hin1 Hin2 Hin3 Hin Hres. intros j' Hlt. 
+        eapply val_rel_rename_ext;
+          [| rewrite <- (compose_id_neut_r (b2 ∘ b')); reflexivity ]. 
+        eapply IHj; [ eassumption | | reflexivity | | | ]. 
+        unfold  val_rel. rewrite <- val_log_rel_eq; tci.
+        clear. now firstorder. now eapply Hres.
+        eapply injective_subdomain_antimon. eassumption.
+        rewrite (reach_unfold _ [set b' l1]).
+        eapply Included_Union_preserv_r.
+        eapply reach'_set_monotonic. simpl. rewrite post_Singleton; [| eassumption ].
+        eapply In_Union_list. eapply in_map. eassumption.
+    - intros Hrel Hres1 Hinj1 Hres2 Hinj2. 
+      destruct v1' as [l1' | lf1' f1']; destruct v2' as [l2' | lf2' f2'];
+        try (rewrite res_equiv_eq in Hres2;
+             rewrite res_equiv_eq in Hres1; contradiction).
+      rewrite res_equiv_eq in Hres2; rewrite res_equiv_eq in Hres1.
+      simpl in Hres1, Hres2.
+      inv Hres1. inv Hres2.
+      eassumption. 
+  Qed.
   
+  Lemma var_rel_heap_env_equiv GP GIP (S1 S2 : Ensemble var) (k j : nat)
+        (β β1 β2 : Inj)
+        (H1 H2 H1' H2' : heap block)
+        (rho1 rho2 rho1' rho2' : env) (x1 x2 : var) :
+    var_rel k j GIP GP β H1 rho1 H2 rho2 x1 x2 ->
+    S1 |- (H1, rho1) ⩪_(id, β1) (H1', rho1') ->
+    injective_subdomain (reach' H1' (env_locs rho1' S1)) β1 -> 
+    S2 |- (H2, rho2) ⩪_(β2, id) (H2', rho2') ->
+    injective_subdomain (reach' H2 (env_locs rho2 S2)) β2 ->
+    x1 \in S1 -> x2 \in S2 ->
+    var_rel k j GIP GP (β2 ∘ β ∘ β1)
+                      H1' rho1' H2' rho2' x1 x2.
+  Proof.
+    intros Henv Heq1 Hinj1 Heq2 Hinj2 Hin1 Hin2 v1' Hget1'.
+    assert (Hget1'' := Hget1').
+    eapply Heq1 in Hget1'; [| eassumption ].
+    destruct Hget1' as [v1 [Hget1 Hequiv1]]. 
+    eapply Henv in Hget1. 
+    destruct Hget1 as [v2 [Hget2 Hval]]; eauto.
+    assert (Hget2'' := Hget2).
+    eapply Heq2 in Hget2; [| eassumption ].
+    destruct Hget2 as [v2' [Hget2' Hequiv2]]; eauto. 
+    eexists. split; eauto.
+    eapply val_rel_res_eq; try eassumption.
+    symmetry. eassumption. 
+    eapply injective_subdomain_antimon. eassumption.
+    eapply reach'_set_monotonic. now eapply get_In_env_locs; eauto.
+    eapply injective_subdomain_antimon. eassumption.
+    eapply reach'_set_monotonic. now eapply get_In_env_locs; eauto.
+  Qed. 
+  
+
+  Lemma env_rel_heap_env_equiv GIP GP (S S1 S2 : Ensemble var) (k j : nat)
+        (b b1 b2 : Inj)
+        (H1 H2 H1' H2' : heap block) (rho1 rho2 rho1' rho2' : env) :
+    (H1, rho1) ⋞ ^ (S; k; j; GIP; GP; b ) (H2, rho2) ->
+    S1 |- (H1, rho1) ⩪_(id, b1) (H1', rho1') ->
+    injective_subdomain (reach' H1' (env_locs rho1' S1)) b1 -> 
+    S2 |- (H2, rho2) ⩪_(b2, id) (H2', rho2') ->
+    injective_subdomain (reach' H2 (env_locs rho2 S2)) b2 ->
+    S \subset S1 -> S \subset S2 ->
+    (H1', rho1') ⋞ ^ (S; k; j; GIP; GP; (b2 ∘ b ∘ b1)) (H2', rho2').
+  Proof.
+    intros Henv Heq1 Hinj1 Heq2 Hinj2 Hin1 Hin2 v1' Hget1'.
+    eapply var_rel_heap_env_equiv; try eassumption; eauto.
+    eapply Henv. eassumption. 
+  Qed.
+  
+  (* Reachable values are in the LR *)
+  
+  Lemma val_rel_post GIP GP (k j : nat) b v1 v2 H1 H2 l :
+    Res (v1, H1) ≺ ^ (k; S j; GIP ; GP; b) Res (v2, H2) ->
+    l \in post H1 (val_loc v1) ->
+    Res (Loc l, H1) ≺ ^ (k; j; GIP ; GP; b) Res (Loc (b l), H2).
+  Proof. 
+    intros Hcc [l' [b' [Hin [Hget Hin']]]].
+    destruct v1 as [l1 |]; [| now inv Hin ]. inv Hin.
+    destruct v2 as [l2 |]; [| now inv Hcc ].
+    destruct Hcc as [Heq Hcc].
+    rewrite Hget in Hcc.
+    
+    (destruct b' as [| |]; try contradiction;
+     destruct (get l2 H2) as [[| |] | ] eqn:Hget'); try contradiction.
+
+    - simpl in  Hin'.      
+      destruct Hcc as [Heq1 Hrel]. subst.
+      simpl in Hrel.
+      edestruct (@Union_lists_exists loc) as [S' [Hin3 Hin2]]. eassumption.
+      edestruct (list_in_map_inv _ _ _ Hin3) as [l3' [Heql Hinl]]; subst.
+      destruct l3' as [l3' |]; inv Hin2.
+      edestruct (Forall2_exists _ l0 l1 (Loc l) Hinl Hrel)  as [x' [Hin2 Hres']].
+      specialize (Hres' j (NPeano.Nat.lt_succ_diag_r j)).
+      rewrite val_log_rel_eq in Hres'; tci.
+      assert (Hleq : x' = Loc (b l)) by (eapply val_log_rel_loc_eq; eauto).
+      subst. eassumption.
+  Qed.
+
+  Lemma val_rel_post_n GIP GP (k j : nat) b v1 v2 H1 H2 l n :
+    Res (v1, H1) ≺ ^ (k; n + j; GIP ; GP; b) Res (v2, H2) ->
+    l \in (post H1 ^ n) (val_loc v1) ->
+    Res (Loc l, H1) ≺ ^ (k; j; GIP ; GP; b ) Res (Loc (b l), H2).
+  Proof.
+    revert v1 v2 l j; induction n as [n IHn] using lt_wf_rec1;
+      destruct n; intros v1 v2 l j. 
+    - intros Heq Hin. destruct v1; [| now inv Hin ]. inv Hin. 
+      erewrite <- !(val_log_rel_loc_eq) with (v2 := v2); eauto.
+    - intros Hrel Hpost.
+      replace (S n) with (n + 1) in Hpost by omega.
+      rewrite app_plus in Hpost. unfold compose in Hpost. simpl in Hpost.
+      edestruct post_n_exists_Singleton as [l3 [Hin1 Hinp]]; try eassumption.
+      eapply IHn with (v1 := Loc l3); [| | eassumption ]. omega.
+      eapply val_rel_post. eassumption. 
+      eassumption. 
+  Qed.
+  
+
+  Corollary val_rel_reach GIP GP (k : nat) b v1 v2 H1 H2 l :
+    (forall j, Res (v1, H1) ≺ ^ (k; j; GIP ; GP; b) Res (v2, H2)) ->
+    l \in reach' H1 (val_loc v1) ->
+    (forall j, Res (Loc l, H1) ≺ ^ (k; j; GIP ; GP; b ) Res (Loc (b l), H2)).
+  Proof.
+    intros Hres [n [_ Hin]] j. eapply val_rel_post_n; now eauto.
+  Qed.
+
   (** * Well-formedness/closedness lemmas *)
 
+  Lemma val_rel_well_formed_post GIP GP (k j : nat) b v1 v2 H1 H2 :
+    Res (v1, H1) ≺ ^ (k; j + 1; GIP ; GP; b) Res (v2, H2) ->
+    well_formed (((post H1) ^ j) (val_loc v1)) H1.
+  Proof.
+    intros Hcc l1 b1 Hin Hget l Hlin.
+    assert (Hp : (post H1 ^ S j) (val_loc v1) l).
+    { simpl. do 2 eexists. split. eassumption. 
+      split; eassumption. }
+    eapply val_rel_post_n with (j := 0) in Hp.
+    eapply val_log_rel_in_dom1. eassumption. 
+    reflexivity.
+    eapply val_rel_j_monotonic; tci. omega.
+  Qed.
+  
+  Lemma val_rel_well_formed_reach GIP GP (k : nat) b v1 v2 H1 H2 :
+    (forall j, Res (v1, H1) ≺ ^ (k; j; GIP ; GP; b) Res (v2, H2)) ->
+    well_formed (reach' H1 (val_loc v1)) H1.
+  Proof.
+    intros Hcc l1 b1 [n [_ Hin]] Hget l Hdom.
+    eapply val_rel_well_formed_post; try eassumption.
+    now eauto.
+  Qed.
+
+  Lemma val_rel_closed GIP GP (k : nat) b v1 v2 H1 H2 :
+    (forall j, Res (v1, H1) ≺ ^ (k; j; GIP ; GP; b) Res (v2, H2)) ->
+    closed (reach' H1 (val_loc v1)) H1.
+  Proof.
+    intros Hyp. eapply reach'_closed.
+    eapply val_rel_well_formed_reach. eassumption.
+    eapply val_log_rel_in_dom1. eapply (Hyp 0). 
+  Qed.
+
+
+  Lemma var_rel_well_formed_reach GP GIP (k : nat)
+        (b : Inj) (H1 H2 : heap block) (rho1 rho2 : env) (x1 x2 : var) :
+    (forall j, var_rel k j GIP GP b H1 rho1 H2 rho2 x1 x2) ->
+    well_formed (reach' H1 (env_locs rho1 [set x1])) H1.
+  Proof.
+    intros Hrel.
+    destruct (M.get x1 rho1) eqn:Heqb.
+    rewrite env_locs_Singleton; eauto.
+    
+    edestruct (Hrel 0) as [v2 [Hget2 Hequiv2]]. eassumption. 
+    eapply val_rel_well_formed_reach. intros j1.
+    edestruct (Hrel j1) as [v2' [Hget2' Hequiv2']]. eassumption. 
+    repeat subst_exp. eassumption.
+
+    rewrite env_locs_Singleton_None; try eassumption. 
+    rewrite reach'_Empty_set. eapply well_formed_Empty_set.
+  Qed.  
+  
+  Lemma var_rel_closed_reach GP GIP (S1 S2 : Ensemble var) (k j : nat)
+        (b : Inj) (H1 H2 H1' H2' : heap block)
+        (rho1 rho2 rho1' rho2' : env) (x1 x2 : var) :
+    (forall j, var_rel k j GIP GP b H1 rho1 H2 rho2 x1 x2) ->
+    closed (reach' H1 (env_locs rho1 [set x1])) H1.
+  Proof.
+    intros Hvar.
+    eapply reach'_closed.     
+    eapply var_rel_well_formed_reach. eassumption.
+
+    destruct (M.get x1 rho1) eqn:Heqb.
+    rewrite env_locs_Singleton; eauto.
+    
+    edestruct (Hvar 0) as [v2 [Hget2 Hequiv2]]. eassumption. 
+    now eapply val_log_rel_in_dom1; eauto.
+    rewrite env_locs_Singleton_None; try eassumption.
+    now eauto with Ensembles_DB. 
+  Qed.  
+    
+  Lemma env_rel_well_fomed_reach GIP GP (P : Ensemble var) (k : nat)
+        (b : Inj) (H1 H2 : heap block) (rho1 rho2 : env) :
+    (forall j, (H1, rho1) ⋞ ^ (P; k; j; GIP; GP; b ) (H2, rho2)) ->
+    well_formed (reach' H1 (env_locs rho1 P)) H1.
+  Proof.
+    intros Henv l1 b1 [n [_ Hin]] Hget l Hlocs. 
+    edestruct post_n_exists_Singleton as [l1' [Hin' Hp]]. eassumption.
+    edestruct Hin' as [y [Hiny Heqy]].
+    destruct (M.get y rho1) as [[l1'' |] |] eqn:Hgety; try contradiction.
+    inv Heqy. eapply Henv with (j := n + 1) in Hgety; [| eassumption ].
+    edestruct Hgety as [l2 [Hgetyl1 Hres]]. 
+    assert (Hr : In loc ((post H1 ^ (S n)) [set l1']) l). 
+    { do 2 eexists; split. eassumption. split; eauto. }
+    eapply val_rel_well_formed_post; eassumption.
+  Qed.
+
+  Lemma env_rel_closed_reach GIP GP (P : Ensemble var) (k : nat)
+        (b : Inj) (H1 H2 : heap block) (rho1 rho2 : env) :
+    (forall j, (H1, rho1) ⋞ ^ (P; k; j; GIP; GP; b ) (H2, rho2)) ->
+    closed (reach' H1 (env_locs rho1 P)) H1.
+  Proof.
+    intros Henv. eapply reach'_closed.
+    eapply env_rel_well_fomed_reach. eassumption.
+    eapply env_log_rel_P_in_dom1. eapply (Henv 0).
+  Qed.
+
+  Lemma heap_rel_well_fomed_reach GIP GP (P : Ensemble var) (k : nat)
+        (b : Inj) (H1 H2 : heap block) :
+    (forall j, P |- H1 ≼ ^ ( k ; j ; GIP ; GP ; b ) H2) ->
+    well_formed (reach' H1 P) H1.
+  Proof.
+    intros Henv l1 b1 [n [_ Hin]] Hget l Hlocs. 
+    edestruct post_n_exists_Singleton as [l1' [Hin' Hp]]. eassumption.
+    eapply val_rel_well_formed_post. eapply Henv. eassumption. simpl. eassumption.
+    eassumption. eassumption.
+  Qed.
+
+  Lemma heap_rel_closed_reach GIP GP (P : Ensemble var) (k : nat)
+        (b : Inj) (H1 H2 : heap block) (rho1 rho2 : env) :
+    (forall j, P |- H1 ≼ ^ ( k ; j ; GIP ; GP ; b ) H2) ->
+    closed (reach' H1 P) H1.
+  Proof.
+    intros Henv. eapply reach'_closed.
+    eapply heap_rel_well_fomed_reach. eassumption.
+    eapply heap_log_rel_in_dom1. eapply (Henv 0).
+  Qed.
+ 
+
+              
   (** * Heap monotonicity/allocation  *)
   
   (** * Reachable locations image *)
